Boolean, computational equality for Sty, Msg, Var
Plus some lemmas concerning decidability of equality of the same types.

SessionTypes.v
@@ -1,4 +1,4 @@
-Require Import Msg Var.
+Require Import Msg Tac Var.
 
 Inductive Sty : Set :=
 | unit : Sty
@@ -8,4 +8,23 @@ Inductive Sty : Set :=
 | ichoice : Sty -> Sty -> Sty
 | mu : Var -> Sty -> Sty
 | var : Var -> Sty
+.
+
+Lemma eq_Sty_dec :
+  forall (S T : Sty), {S = T} + {S <> T}.
+Proof.
+  pose proof eq_Msg_dec. pose proof eq_var_dec. decide equality; auto.
+Defined.
+
+Fixpoint beq_Sty (S T : Sty) : bool :=
+  match (S, T) with
+  | (unit, unit) => true
+  | (send B S', send B' T') => andb (beq_msg B B') (beq_Sty S' T')
+  | (recv B S', recv B' T') => andb (beq_msg B B') (beq_Sty S' T')
+  | (echoice S1 S2, echoice T1 T2) => andb (beq_Sty S1 T1) (beq_Sty S2 T2)
+  | (ichoice S1 S2, ichoice T1 T2) => andb (beq_Sty S1 T1) (beq_Sty S2 T2)
+  | (mu X S', mu Y T') => andb (beq_var X Y) (beq_Sty S' T')
+  | (var X, var Y) => beq_var X Y
+  | _ => false
+  end
 .
