Msg.v
@@ -9,3 +9,7 @@ Definition beq_msg x y :=
   | (mkMsg x, mkMsg y) => beq_nat x y
   end
 .
+
+Lemma eq_Msg_dec :
+  forall (M M' : Msg), {M = M'} + {M <> M'}.
+Proof. decide equality. apply eq_nat_dec. Defined.
